IsaSAT: starting to add LLVM code generation

Weidenbach_Book/IsaSAT_Initialisation.thy
@@ -252,7 +252,7 @@ definition initialise_VMTF :: \<open>uint32 list \<Rightarrow> nat \<Rightarrow>
         let L = nat_of_uint32 (N ! i);
         ASSERT(L < length A);
         ASSERT(cnext \<noteq> None \<longrightarrow> the cnext < length A);
-        ASSERT(i + 1 \<le> uint_max);
+        ASSERT(i + 1 \<le> uint32_max);
         RETURN (i + one_uint32_nat, vmtf_cons A L cnext (uint64_of_uint32_conv i), Some L)
       })
       (zero_uint32_nat, A, None);
@@ -282,7 +282,7 @@ proof -
               let L = nat_of_uint32 (N' ! i);
               _ \<leftarrow> ASSERT (L < length A);
               _ \<leftarrow> ASSERT (cnext \<noteq> None \<longrightarrow> the cnext < length A);
-              _ \<leftarrow> ASSERT (i + 1 \<le> uint_max);
+              _ \<leftarrow> ASSERT (i + 1 \<le> uint32_max);
               RETURN
                (i + one_uint32_nat,
                 vmtf_cons A L cnext (uint64_of_uint32_conv i), Some L)
@@ -623,7 +623,7 @@ definition add_init_cls_heur
   :: \<open>bool \<Rightarrow> nat clause_l \<Rightarrow> twl_st_wl_heur_init \<Rightarrow> twl_st_wl_heur_init nres\<close>  where
   \<open>add_init_cls_heur unbdd = (\<lambda>C (M, N, D, Q, W, vm, \<phi>, clvls, cach, lbd, vdom, failed). do {
      let C = C;
-     ASSERT(length C \<le> uint_max + 2);
+     ASSERT(length C \<le> uint32_max + 2);
      ASSERT(length C \<ge> 2);
      if unbdd \<or> (length N \<le> uint64_max - length C - 5 \<and> \<not>failed)
      then do {
@@ -802,8 +802,8 @@ nat list \<times> bool list) \<times>
       \<open>x = (x1g, x2g)\<close>
 begin
 
-lemma add_init_pre1: \<open>length x1g \<le> uint_max + 2\<close>
-  using pre clss_size_uint_max[of \<A> \<open>mset x1g\<close>] xy st
+lemma add_init_pre1: \<open>length x1g \<le> uint32_max + 2\<close>
+  using pre clss_size_uint32_max[of \<A> \<open>mset x1g\<close>] xy st
   by (auto simp: twl_st_heur_parsing_no_WL_def)
 
 lemma add_init_pre2: \<open>2 \<le> length x1g\<close>
@@ -1180,7 +1180,7 @@ definition isasat_atms_ext_rel :: \<open>((nat list \<times> nat \<times> nat li
   \<open>isasat_atms_ext_rel = {((xs, n, atms), l).
       init_valid_rep xs l \<and>
       n = Max (insert 0 l) \<and>
-      length xs < uint_max \<and>
+      length xs < uint32_max \<and>
       (\<forall>s\<in>set xs. s \<le> uint64_max) \<and>
       finite l \<and>
       distinct atms \<and>
@@ -1204,7 +1204,7 @@ lemma isasat_atms_ext_rel_alt_def:
   \<open>isasat_atms_ext_rel = {((xs, n, atms), l).
       init_valid_rep xs l \<and>
       n = Max (insert 0 l) \<and>
-      length xs < uint_max \<and>
+      length xs < uint32_max \<and>
       (\<forall>s\<in>set xs. s \<le> uint64_max) \<and>
       finite l \<and>
       distinct atms \<and>
@@ -1221,13 +1221,13 @@ definition in_map_atm_of :: \<open>'a \<Rightarrow> 'a list \<Rightarrow> bool\<
 definition (in -) init_next_size where
   \<open>init_next_size L = 2 * L\<close>
 
-lemma init_next_size: \<open>L \<noteq> 0 \<Longrightarrow> L + 1 \<le> uint_max \<Longrightarrow> L < init_next_size L\<close>
-  by (auto simp: init_next_size_def uint32_max_uint32_def uint_max_def)
+lemma init_next_size: \<open>L \<noteq> 0 \<Longrightarrow> L + 1 \<le> uint32_max \<Longrightarrow> L < init_next_size L\<close>
+  by (auto simp: init_next_size_def uint32_max_uint32_def uint32_max_def)
 
 definition add_to_atms_ext where
   \<open>add_to_atms_ext = (\<lambda>i (xs, n, atms). do {
-    ASSERT(i \<le> uint_max div 2);
-    ASSERT(length xs \<le> uint_max);
+    ASSERT(i \<le> uint32_max div 2);
+    ASSERT(length xs \<le> uint32_max);
     ASSERT(length atms \<le> Suc n);
     let n = max i n;
     (if i < length_uint32_nat xs then do {
@@ -1236,7 +1236,7 @@ definition add_to_atms_ext where
        RETURN (xs[i := (sum_mod_uint64_max (xs ! i) 2) OR one_uint64_nat], n, atms)
      }
      else do {
-        ASSERT(i + 1 \<le> uint_max);
+        ASSERT(i + 1 \<le> uint32_max);
         ASSERT(length_uint32_nat xs \<noteq> 0);
         ASSERT(i < init_next_size i);
         RETURN ((list_grow xs (init_next_size i) zero_uint64_nat)[i := one_uint64_nat], n,
@@ -1357,7 +1357,7 @@ lemma init_valid_rep_in_set_iff:
 
 lemma add_to_atms_ext_op_set_insert:
   \<open>(uncurry add_to_atms_ext, uncurry (RETURN oo Set.insert))
-   \<in> [\<lambda>(n, l). n \<le> uint_max div 2]\<^sub>f nat_rel \<times>\<^sub>f isasat_atms_ext_rel \<rightarrow> \<langle>isasat_atms_ext_rel\<rangle>nres_rel\<close>
+   \<in> [\<lambda>(n, l). n \<le> uint32_max div 2]\<^sub>f nat_rel \<times>\<^sub>f isasat_atms_ext_rel \<rightarrow> \<langle>isasat_atms_ext_rel\<rangle>nres_rel\<close>
 proof -
   have H: \<open>finite x2 \<Longrightarrow> Max (insert x1 (insert 0 x2)) = Max (insert x1 x2)\<close>
     \<open>finite x2 \<Longrightarrow> Max (insert 0 (insert x1 x2)) = Max (insert x1 x2)\<close>
@@ -1401,9 +1401,9 @@ proof -
       subgoal
         by (auto simp add: init_valid_rep_in_set_iff)
       done
-    subgoal by (auto simp: uint_max_def)
-    subgoal by (auto simp: uint_max_def)
-    subgoal by (auto simp: uint_max_def init_next_size_def elim: neq_NilE)
+    subgoal by (auto simp: uint32_max_def)
+    subgoal by (auto simp: uint32_max_def)
+    subgoal by (auto simp: uint32_max_def init_next_size_def elim: neq_NilE)
     subgoal
       unfolding comp_def list_grow_def
       apply (rule RETURN_refine)
@@ -1419,7 +1419,7 @@ proof -
         apply (auto elim: neq_NilE)
         done
       subgoal by (auto simp: H Max_insert[symmetric] simp del: Max_insert)
-      subgoal by (auto simp: init_next_size_def uint_max_def)
+      subgoal by (auto simp: init_next_size_def uint32_max_def)
       subgoal
         using sum_mod_uint64_max_le_uint64_max
         unfolding bitOR_1_if_mod_2_nat one_uint64_nat_def
@@ -1440,7 +1440,7 @@ definition extract_atms_cls :: \<open>'a clause_l \<Rightarrow> 'a set \<Rightar
 definition extract_atms_cls_i :: \<open>nat clause_l \<Rightarrow> nat set \<Rightarrow> nat set nres\<close> where
   \<open>extract_atms_cls_i C \<A>\<^sub>i\<^sub>n = nfoldli C (\<lambda>_. True)
        (\<lambda>L \<A>\<^sub>i\<^sub>n. do {
-         ASSERT(atm_of L \<le> uint_max div 2);
+         ASSERT(atm_of L \<le> uint32_max div 2);
          RETURN(insert (atm_of L) \<A>\<^sub>i\<^sub>n)})
     \<A>\<^sub>i\<^sub>n\<close>
 
@@ -1453,12 +1453,12 @@ lemma extract_atms_cls_alt_def: \<open>extract_atms_cls C \<A>\<^sub>i\<^sub>n =
 
 lemma extract_atms_cls_i_extract_atms_cls:
   \<open>(uncurry extract_atms_cls_i, uncurry (RETURN oo extract_atms_cls))
-   \<in> [\<lambda>(C, \<A>\<^sub>i\<^sub>n). \<forall>L\<in>set C. nat_of_lit L \<le> uint_max]\<^sub>f
+   \<in> [\<lambda>(C, \<A>\<^sub>i\<^sub>n). \<forall>L\<in>set C. nat_of_lit L \<le> uint32_max]\<^sub>f
      \<langle>Id\<rangle>list_rel \<times>\<^sub>f Id \<rightarrow> \<langle>Id\<rangle>nres_rel\<close>
 proof -
-  have H1: \<open>(x1a, x1) \<in> \<langle>{(L, L'). L = L' \<and> nat_of_lit L \<le> uint_max}\<rangle>list_rel\<close>
+  have H1: \<open>(x1a, x1) \<in> \<langle>{(L, L'). L = L' \<and> nat_of_lit L \<le> uint32_max}\<rangle>list_rel\<close>
     if
-      \<open>case y of (C, \<A>\<^sub>i\<^sub>n) \<Rightarrow>  \<forall>L\<in>set C. nat_of_lit L \<le> uint_max\<close> and
+      \<open>case y of (C, \<A>\<^sub>i\<^sub>n) \<Rightarrow>  \<forall>L\<in>set C. nat_of_lit L \<le> uint32_max\<close> and
       \<open>(x, y) \<in> \<langle>nat_lit_lit_rel\<rangle>list_rel \<times>\<^sub>f Id\<close> and
       \<open>y = (x1, x2)\<close> and
       \<open>x = (x1a, x2a)\<close>
@@ -1466,8 +1466,8 @@ proof -
       x1 :: \<open>nat literal list\<close> and x2 :: \<open>nat set\<close> and x1a :: \<open>nat literal list\<close> and x2a :: \<open>nat set\<close>
     using that by (auto simp: list_rel_def list_all2_conj list.rel_eq list_all2_conv_all_nth)
 
-  have atm_le: \<open>nat_of_lit xa \<le> uint_max \<Longrightarrow> atm_of xa \<le> uint_max div 2\<close> for xa
-    by (cases xa) (auto simp: uint_max_def)
+  have atm_le: \<open>nat_of_lit xa \<le> uint32_max \<Longrightarrow> atm_of xa \<le> uint32_max div 2\<close> for xa
+    by (cases xa) (auto simp: uint32_max_def)
 
   show ?thesis
     supply RETURN_as_SPEC_refine[refine2 del]
@@ -1493,12 +1493,12 @@ definition extract_atms_clss_i :: \<open>nat clause_l list \<Rightarrow> nat set
 
 lemma extract_atms_clss_i_extract_atms_clss:
   \<open>(uncurry extract_atms_clss_i, uncurry (RETURN oo extract_atms_clss))
-   \<in> [\<lambda>(N, \<A>\<^sub>i\<^sub>n). \<forall>C\<in>set N. \<forall>L\<in>set C. nat_of_lit L \<le> uint_max]\<^sub>f
+   \<in> [\<lambda>(N, \<A>\<^sub>i\<^sub>n). \<forall>C\<in>set N. \<forall>L\<in>set C. nat_of_lit L \<le> uint32_max]\<^sub>f
      \<langle>Id\<rangle>list_rel \<times>\<^sub>f Id \<rightarrow> \<langle>Id\<rangle>nres_rel\<close>
 proof -
-  have H1: \<open>(x1a, x1) \<in> \<langle>{(C, C'). C = C' \<and> (\<forall>L\<in>set C. nat_of_lit L \<le> uint_max)}\<rangle>list_rel\<close>
+  have H1: \<open>(x1a, x1) \<in> \<langle>{(C, C'). C = C' \<and> (\<forall>L\<in>set C. nat_of_lit L \<le> uint32_max)}\<rangle>list_rel\<close>
     if
-      \<open>case y of (N, \<A>\<^sub>i\<^sub>n) \<Rightarrow> \<forall>C\<in>set N. \<forall>L\<in>set C. nat_of_lit L \<le> uint_max\<close> and
+      \<open>case y of (N, \<A>\<^sub>i\<^sub>n) \<Rightarrow> \<forall>C\<in>set N. \<forall>L\<in>set C. nat_of_lit L \<le> uint32_max\<close> and
       \<open>(x, y) \<in> \<langle>Id\<rangle>list_rel \<times>\<^sub>f Id\<close> and
       \<open>y = (x1, x2)\<close> and
       \<open>x = (x1a, x2a)\<close>
@@ -1546,7 +1546,7 @@ lemma extract_atms_clss_imp_empty_rel:
   \<open>(\<lambda>_. extract_atms_clss_imp_empty_rel, \<lambda>_. (RETURN op_extract_list_empty)) \<in>
      unit_rel \<rightarrow>\<^sub>f \<langle>isasat_atms_ext_rel\<rangle> nres_rel\<close>
   by (intro frefI nres_relI)
-    (simp add:  op_extract_list_empty_def uint_max_def
+    (simp add:  op_extract_list_empty_def uint32_max_def
       isasat_atms_ext_rel_def init_valid_rep_def extract_atms_clss_imp_empty_rel_def
        del: replicate_numeral)
 
@@ -1912,20 +1912,20 @@ proof -
   have K: \<open>RETURN o mset_set = (\<lambda>v. do {v' \<leftarrow> SPEC(\<lambda>v'. v' = mset_set v); RETURN v'})\<close>
     by auto
   have K': \<open>length x2a < uint32_max\<close> if \<open>distinct b\<close> \<open>init_valid_rep x1 (set b)\<close>
-    \<open>length x1 < uint_max\<close> \<open>mset x2a = mset b\<close>for x1 x2a b
+    \<open>length x1 < uint32_max\<close> \<open>mset x2a = mset b\<close>for x1 x2a b
   proof -
     have \<open>distinct x2a\<close>
       by (simp add: same_mset_distinct_iff that(1) that(4))
     have \<open>length x2a = length b\<close> \<open>set x2a = set b\<close>
       using \<open>mset x2a = mset b\<close> apply (metis size_mset)
        using \<open>mset x2a = mset b\<close> by (rule mset_eq_setD)
-    then have \<open>set x2a \<subseteq> {0..<uint_max - 1}\<close>
+    then have \<open>set x2a \<subseteq> {0..<uint32_max - 1}\<close>
       using that by (auto simp: init_valid_rep_def)
     from card_mono[OF _ this] show ?thesis
-      using \<open>distinct x2a\<close> by (auto simp: uint_max_def distinct_card)
+      using \<open>distinct x2a\<close> by (auto simp: uint32_max_def distinct_card)
   qed
   have H_simple: \<open>RETURN x2a
-      \<le> \<Down> (list_mset_rel \<inter> {(v, v'). length v < uint_max})
+      \<le> \<Down> (list_mset_rel \<inter> {(v, v'). length v < uint32_max})
           (SPEC (\<lambda>v'. v' = mset_set y))\<close>
     if
       \<open>(x, y) \<in> isasat_atms_ext_rel\<close> and
@@ -2198,7 +2198,7 @@ proof -
 
   have initialise_VMTF: \<open>initialise_VMTF a (Suc (nat_of_uint32 b)) \<le>
        \<Down> Id (RES (isa_vmtf_init y []))\<close>
-    if \<open>(x, y) \<in> ?arg\<close> and \<open>distinct_mset y\<close> and \<open>length a < uint_max\<close> and \<open>x = (a, b)\<close> for x y a b
+    if \<open>(x, y) \<in> ?arg\<close> and \<open>distinct_mset y\<close> and \<open>length a < uint32_max\<close> and \<open>x = (a, b)\<close> for x y a b
     using that
     by (auto simp: P_def lits_with_max_rel_def intro!: initialise_VMTF in_N0)
   have K[simp]: \<open>(x, \<A>\<^sub>i\<^sub>n) \<in> \<langle>uint32_nat_rel\<rangle>list_rel_mset_rel \<Longrightarrow>
@@ -2246,8 +2246,8 @@ proof -
      \<open>NO_MATCH 0 a1 \<Longrightarrow> max 0 (Max (insert a1 (set a2))) = max a1 (Max (insert 0 (set a2)))\<close>
     for a1 :: uint32 and a2
     by (metis (mono_tags, lifting) List.finite_set Max_insert all_not_in_conv finite_insert insertI1 insert_commute)
-  have le_uint32: \<open>\<forall>L\<in>#\<L>\<^sub>a\<^sub>l\<^sub>l (nat_of_uint32 `# mset a). nat_of_lit L \<le> uint_max \<Longrightarrow>
-    Suc (2 * nat_of_uint32 (Max (insert 0 (set a)))) \<le> uint_max\<close> for a
+  have le_uint32: \<open>\<forall>L\<in>#\<L>\<^sub>a\<^sub>l\<^sub>l (nat_of_uint32 `# mset a). nat_of_lit L \<le> uint32_max \<Longrightarrow>
+    Suc (2 * nat_of_uint32 (Max (insert 0 (set a)))) \<le> uint32_max\<close> for a
     apply (induction a)
     apply (auto simp: uint32_max_def)
     apply (auto simp: max_def  \<L>\<^sub>a\<^sub>l\<^sub>l_add_mset)
