Weidenbach_Book/IsaSAT_Clauses_SML.thy
@@ -109,14 +109,14 @@ sepref_definition nth_rll_u64_i64_clauses
 
 sepref_definition length_rll_n_uint32_clss
   is \<open>uncurry (RETURN oo (\<lambda>(N, _) i. length_rll_n_uint32 N i))\<close>
-  :: \<open>[\<lambda>((xs, _), i). i < length xs \<and> length (xs ! i) \<le> uint_max]\<^sub>a
+  :: \<open>[\<lambda>((xs, _), i). i < length xs \<and> length (xs ! i) \<le> uint32_max]\<^sub>a
        isasat_clauses_assn\<^sup>k *\<^sub>a nat_assn\<^sup>k \<rightarrow> uint32_nat_assn\<close>
   by sepref
 
 
 sepref_definition length_raa_i64_u_clss
   is \<open>uncurry (RETURN oo (\<lambda>(N, _) i. length_rll_n_uint32 N i))\<close>
-  :: \<open>[\<lambda>((xs, _), i). i < length xs \<and> length (xs ! i) \<le> uint_max]\<^sub>a
+  :: \<open>[\<lambda>((xs, _), i). i < length xs \<and> length (xs ! i) \<le> uint32_max]\<^sub>a
        isasat_clauses_assn\<^sup>k *\<^sub>a uint64_nat_assn\<^sup>k \<rightarrow> uint32_nat_assn\<close>
   by sepref
 
