Weidenbach_Book/IsaSAT_Decide.thy
@@ -51,7 +51,7 @@ where
      (L = None \<longrightarrow> (\<forall>K\<in># \<L>\<^sub>a\<^sub>l\<^sub>l \<A>. defined_lit M K)) \<and> M = M' \<and> vm \<in> vmtf \<A> M)\<close>
 
 definition lit_of_found_atm_D_pre where
-\<open>lit_of_found_atm_D_pre = (\<lambda>(\<phi>, L). L \<noteq> None \<longrightarrow> (the L < length \<phi> \<and> the L \<le> uint_max div 2))\<close>
+\<open>lit_of_found_atm_D_pre = (\<lambda>(\<phi>, L). L \<noteq> None \<longrightarrow> (the L < length \<phi> \<and> the L \<le> uint32_max div 2))\<close>
 
 definition find_unassigned_lit_wl_D_heur
   :: \<open>twl_st_wl_heur \<Rightarrow> (twl_st_wl_heur \<times> nat literal option) nres\<close>
