Weidenbach_Book/IsaSAT_Restart.thy
@@ -157,7 +157,7 @@ proof -
     by (auto simp: twl_st_heur'_def)
   have H: \<open>(xb, x'a)
     \<in> bool_rel \<times>\<^sub>f
-      twl_st_heur'''' (length (get_clauses_wl_heur x1e) + 6 + uint_max div 2) \<Longrightarrow>
+      twl_st_heur'''' (length (get_clauses_wl_heur x1e) + 6 + uint32_max div 2) \<Longrightarrow>
     x'a = (x1f, x2f) \<Longrightarrow>
     xb = (x1g, x2g) \<Longrightarrow>
     (x1g, x1f) \<in> bool_rel \<Longrightarrow>
@@ -377,7 +377,7 @@ proof -
     by (auto simp: twl_st_heur'_def)
   have H: \<open>(xb, x'a)
     \<in> bool_rel \<times>\<^sub>f
-      twl_st_heur'''' (length (get_clauses_wl_heur x1e) + 6 + uint_max div 2) \<Longrightarrow>
+      twl_st_heur'''' (length (get_clauses_wl_heur x1e) + 6 + uint32_max div 2) \<Longrightarrow>
     x'a = (x1f, x2f) \<Longrightarrow>
     xb = (x1g, x2g) \<Longrightarrow>
     (x1g, x1f) \<in> bool_rel \<Longrightarrow>
