Weidenbach_Book/WB_More_Word.thy
@@ -1,0 +1,54 @@
+theory WB_More_Word
+  imports "HOL-Word.More_Word" Bits_Natural
+begin
+
+lemma nat_uint_XOR: \<open>nat (uint (a XOR b)) = nat (uint a) XOR nat (uint b)\<close>
+  if len: \<open>LENGTH('a) > 0\<close>
+  for a b :: \<open>'a ::len0 Word.word\<close>
+proof -
+  have 1: \<open>uint ((word_of_int:: int \<Rightarrow> 'a Word.word)(uint a)) = uint a\<close>
+    by (subst (2) word_of_int_uint[of a, symmetric]) (rule refl)
+  have H: \<open>nat (bintrunc n (a XOR b)) = nat (bintrunc n a XOR bintrunc n b)\<close>
+    if \<open>n> 0\<close> for n and a :: int and b :: int
+    using that
+  proof (induction n arbitrary: a b)
+    case 0
+    then show ?case by auto
+  next
+    case (Suc n) note IH = this(1) and Suc = this(2)
+    then show ?case
+    proof (cases n)
+      case (Suc m)
+      moreover have
+        \<open>nat (bintrunc m (bin_rest (bin_rest a) XOR bin_rest (bin_rest b)) BIT
+            ((bin_last (bin_rest a) \<or> bin_last (bin_rest b)) \<and>
+             (bin_last (bin_rest a) \<longrightarrow> \<not> bin_last (bin_rest b))) BIT
+            ((bin_last a \<or> bin_last b) \<and> (bin_last a \<longrightarrow> \<not> bin_last b))) =
+         nat ((bintrunc m (bin_rest (bin_rest a)) XOR bintrunc m (bin_rest (bin_rest b))) BIT
+              ((bin_last (bin_rest a) \<or> bin_last (bin_rest b)) \<and>
+               (bin_last (bin_rest a) \<longrightarrow> \<not> bin_last (bin_rest b))) BIT
+              ((bin_last a \<or> bin_last b) \<and> (bin_last a \<longrightarrow> \<not> bin_last b)))\<close>
+        (is \<open>nat (?n1 BIT ?b) = nat (?n2 BIT ?b)\<close>)
+      proof - (* Sledgehammer proof changed to use the more readable ?n1 and ?n2 *)
+        have a1:  "nat ?n1 = nat ?n2"
+          using IH Suc by auto
+        have f2: "0 \<le> ?n2"
+          by (simp add: bintr_ge0)
+        have "0 \<le> ?n1"
+          using bintr_ge0 by auto
+        then have "?n2 = ?n1"
+          using f2 a1 by presburger
+        then show ?thesis by simp
+      qed
+      ultimately show ?thesis by simp
+    qed simp
+  qed
+  have \<open>nat (bintrunc LENGTH('a) (a XOR b)) = nat (bintrunc LENGTH('a) a XOR bintrunc LENGTH('a) b)\<close> for a b
+    using len H[of \<open>LENGTH('a)\<close> a b] by auto
+  then have \<open>nat (uint (a XOR b)) = nat (uint a XOR uint b)\<close>
+    by transfer
+  then show ?thesis
+    unfolding bitXOR_nat_def by auto
+qed
+
+end
